\documentclass[preview]{standalone}

\usepackage[english]{babel}
\usepackage{amsmath}
\usepackage{amssymb}

\begin{document}

\begin{align*}
\
            a \bmod p = k &\implies a = pq + k, \text{for } q \in \mathbb{Z} \\ \
                a\bmod p = b \bmod p &\implies b \bmod p = k\\ \
                &\implies b = p\ell + k, \text{for }\ell \in \mathbb{Z} \\ \
                |A - B| \bmod p &= |pq + k - (p\ell + k)| \bmod p \\ \
                &= |pq - pl| \bmod p \\ \
                &= |p(q - \ell)| \bmod p \\ \
                &\boxed{=0} \\ \
\end{align*}

\end{document}
